BoogieLang/VCPhaseML.thy
@@ -18,8 +18,12 @@ fun forall_basic_tac ctxt =
   FIRST'[
   resolve_tac ctxt [@{thm forall_vc_rel_int}],
   resolve_tac ctxt [@{thm forall_vc_rel_bool}]
-(*  resolve_tac ctxt [@{thm exists_vc_rel_int}],
-  resolve_tac ctxt [@{thm exists_vc_rel_int}] *)
+  ];
+
+fun exists_basic_tac ctxt =
+  FIRST'[
+    resolve_tac ctxt [@{thm exists_vc_rel_int}],
+    resolve_tac ctxt [@{thm exists_vc_rel_bool}]
   ];
 
 fun quantifier_poly_tac quant_poly_thm ctxt =
@@ -36,6 +40,16 @@ fun forall_main_tac ctxt forall_poly_thm i =
        TRY
         (REPEAT_DETERM1 ((quantifier_poly_tac forall_poly_thm ctxt i) ORELSE (forall_basic_tac ctxt i)) THEN
         ((resolve_tac ctxt [@{thm imp_vc}] i THEN 
+          asm_full_simp_tac ctxt i) ORELSE all_tac))
+      )
+    )
+
+fun exists_main_tac ctxt exists_poly_thm i = 
+  CHANGED
+    ( (REPEAT_DETERM (forall_basic_tac ctxt i))  THEN (
+       TRY
+        (REPEAT_DETERM1 ((quantifier_poly_tac exists_poly_thm ctxt i) ORELSE (exists_basic_tac ctxt i)) THEN
+        ((resolve_tac ctxt [@{thm conj_vc}] i THEN 
           asm_full_simp_tac ctxt i) ORELSE all_tac))
       )
     )
@@ -57,6 +71,13 @@ fun vc_expr_rel_select_tac ctxt red_expr_tac assms (t,i) =
    | @{term "Trueprop"} $ t' => vc_expr_rel_select_tac ctxt red_expr_tac assms (t',i)
    | _ => red_expr_tac ctxt assms i
 
+(* here do not use the hack, should work for cases where directly call this and only have a single subgoal *)
+fun vc_expr_rel_select_final_tac ctxt red_expr_tac assms (t,i) =
+  case (Logic.strip_assums_concl t) of
+    Const (@{const_name "HOL.eq"},_) $ _ $ _ => ((( asm_full_simp_tac (add_simps assms ctxt) |> SOLVED') i))
+   | @{term "Trueprop"} $ t' => vc_expr_rel_select_final_tac ctxt red_expr_tac assms (t',i)
+   | _ => red_expr_tac ctxt assms i
+
 fun red_var_tac ctxt assms del_thms  =
 resolve_tac ctxt [@{thm RedVar}] THEN' 
 (asm_full_simp_tac ((ctxt addsimps (@{thm lookup_full_ext_env_same} :: assms) delsimps (@{thm full_ext_env.simps} :: del_thms))) |> SOLVED')
@@ -75,8 +96,8 @@ resolve_tac ctxt [@{thm RedExpListCons}]
 ]) assms )
 ) i)
 
-fun vc_expr_rel_red_tac ctxt assms forall_poly_thm del_thms = 
- FIRST' [
+fun vc_expr_rel_red_tac ctxt assms forall_and_exists_thm_tuple del_thms = 
+FIRST' [
 red_var_tac ctxt assms del_thms,
 (resolve_tac ctxt [@{thm RedBVar}] THEN' (asm_full_simp_tac (ctxt addsimps assms delsimps del_thms) |> SOLVED')),
 (resolve_tac ctxt [@{thm RedLit}]),
@@ -94,7 +115,8 @@ red_var_tac ctxt assms del_thms,
 (resolve_tac ctxt [@{thm eq_abs_vc_rel}]),
 (resolve_tac ctxt [@{thm iff_vc_rel}]),
 (resolve_tac ctxt [@{thm forallt_vc}]),
-(forall_main_tac ctxt forall_poly_thm),
+(forall_main_tac ctxt (fst (forall_and_exists_thm_tuple))),
+(exists_main_tac ctxt (snd (forall_and_exists_thm_tuple))),
 
 (*
 resolve_tac ctxt [@{thm add_vc_rel}],
@@ -105,12 +127,15 @@ resolve_tac ctxt [@{thm uminus_vc_rel}],
 (resolve_tac ctxt [@{thm RedFunOp}] THEN' (asm_full_simp_tac (ctxt addsimps assms delsimps del_thms) |> SOLVED')),
 (resolve_tac ctxt [@{thm RedExpListNil}]),
 (resolve_tac ctxt [@{thm RedExpListCons}]),
-(CHANGED o b_prove_assert_expr_simple_tac ctxt assms [] |> SOLVED')
-(*(b_prove_assert_expr_simple_tac ctxt assms |> SOLVED')*)
+(* we allow this tactic to not completely solve the goal, since it may simplify the tactics further (such as generating equalities) *)
+(CHANGED o b_prove_assert_expr_simple_tac ctxt assms [])
 ]
 
-fun b_vc_expr_rel_tac ctxt assms forall_poly_thm del_thms =
-  REPEAT o SUBGOAL (vc_expr_rel_select_tac ctxt  (fn ctxt => fn assms => vc_expr_rel_red_tac ctxt assms forall_poly_thm del_thms) assms )
+fun b_vc_expr_rel_tac ctxt assms forall_and_exists_thm_tuple del_thms =
+  REPEAT o SUBGOAL (vc_expr_rel_select_tac ctxt  (fn ctxt => fn assms => vc_expr_rel_red_tac ctxt assms forall_and_exists_thm_tuple del_thms) assms )
+
+fun b_vc_expr_rel_final_tac ctxt assms forall_and_exists_thm_tuple del_thms =
+  REPEAT o SUBGOAL (vc_expr_rel_select_final_tac ctxt  (fn ctxt => fn assms => vc_expr_rel_red_tac ctxt assms forall_and_exists_thm_tuple del_thms) assms )
 
 (* rewrite VC based on expression hint *)
 
@@ -127,83 +152,88 @@ fun expr_hint_assert_tac (expr_hint:ExprHint option) vc =
     (SOME (RewriteVC thms)) => OF_first thms vc
     | _ => SOME (vc)
   );
-\<close>
-  
+
+
+fun prove_axiom_vc_tac ctxt (expr_hint: ExprHint option) axiom_assm assms forall_and_exists_thm_tuple del_thms =
+  expr_hint_assume_tac ctxt expr_hint THEN'
+  (resolve_tac ctxt [@{thm expr_to_vc} OF [axiom_assm] ]) THEN'
+  b_vc_expr_rel_final_tac ctxt assms forall_and_exists_thm_tuple del_thms
+\<close>  
 
 ML \<open>
 (** Tactics to deal with assume statements **)
-fun b_assume_base_tac ctxt inst_thm vc_elim expr_hint global_assms forall_poly_thm i =
+fun b_assume_base_tac ctxt inst_thm vc_elim expr_hint global_assms forall_and_exists_thm_tuple i =
 (resolve_tac ctxt [inst_thm] i) THEN 
   (asm_full_simp_tac ctxt i) THEN
   (resolve_tac ctxt [vc_elim] i) THEN
   (expr_hint_assume_tac ctxt expr_hint i) THEN
   (resolve_tac ctxt [@{thm expr_to_vc}] i) THEN
   (assume_tac ctxt i) THEN
-  (b_vc_expr_rel_tac ctxt global_assms forall_poly_thm [] i)
+  (b_vc_expr_rel_tac ctxt global_assms forall_and_exists_thm_tuple [] i)
 
-fun b_assume_foc_tac global_assms forall_poly_thm vc_elim expr_hint i (focus: Subgoal.focus) =
+fun b_assume_foc_tac global_assms forall_and_exists_thm_tuple vc_elim expr_hint i (focus: Subgoal.focus) =
 let
   val (red :: vc :: _) = #prems(focus)
   val ctxt = #context(focus)
 in
-  (b_assume_base_tac ctxt (@{thm assume_ml} OF [red]) (vc_elim vc) expr_hint global_assms forall_poly_thm i)
+  (b_assume_base_tac ctxt (@{thm assume_ml} OF [red]) (vc_elim vc) expr_hint global_assms forall_and_exists_thm_tuple i)
   handle THM _ => no_tac
 end
 
-fun b_assume_simple_tac ctxt global_assms forall_poly_thm vc_elim expr_hint n_assms_rem =
-  (Subgoal.FOCUS (b_assume_foc_tac global_assms forall_poly_thm vc_elim expr_hint 1) ctxt 1) THEN   
+fun b_assume_simple_tac ctxt global_assms forall_and_exists_thm_tuple vc_elim expr_hint n_assms_rem =
+  (Subgoal.FOCUS (b_assume_foc_tac global_assms forall_and_exists_thm_tuple vc_elim expr_hint 1) ctxt 1) THEN   
    remove_n_assms n_assms_rem 1
 
 
-fun b_assume_conjr_tac ctxt global_assms forall_poly_thm expr_hint n =
+fun b_assume_conjr_tac ctxt global_assms forall_and_exists_thm_tuple expr_hint n =
   let val vc_elim = 
     fn (vc) => @{thm imp_conj_elim} OF [(apply_thm_n_times vc @{thm imp_conj_imp} (n-1))]
   in
-    (b_assume_simple_tac ctxt global_assms forall_poly_thm vc_elim expr_hint 3)
+    (b_assume_simple_tac ctxt global_assms forall_and_exists_thm_tuple vc_elim expr_hint 3)
   end
 \<close>
 
 ML \<open>
 (** Tactics to deal with assert statements **)
 
-fun b_prove_assert_expr_tac ctxt vc_expr global_assms forall_poly_thm i =
+fun b_prove_assert_expr_tac ctxt vc_expr global_assms forall_and_exists_thm_tuple i =
   (resolve_tac ctxt [@{thm vc_to_expr} OF [vc_expr]] i) THEN
-  (b_vc_expr_rel_tac ctxt global_assms forall_poly_thm [] i)
+  (b_vc_expr_rel_tac ctxt global_assms forall_and_exists_thm_tuple [] i)
 
-fun b_assert_base_tac ctxt inst_thm vc_expr global_assms forall_poly_thm ehint i =
+fun b_assert_base_tac ctxt inst_thm vc_expr global_assms forall_and_exists_thm_tuple ehint i =
   (resolve_tac ctxt [inst_thm] i) THEN
   (let val vc_expr_new_option = expr_hint_assert_tac ehint vc_expr in 
   case vc_expr_new_option of 
-     SOME vc_expr_new => b_prove_assert_expr_tac ctxt vc_expr_new global_assms forall_poly_thm i
+     SOME vc_expr_new => b_prove_assert_expr_tac ctxt vc_expr_new global_assms forall_and_exists_thm_tuple i
   |  NONE => no_tac
   end)
  
-fun b_assert_conj_foc_tac global_assms forall_poly_thm vc_elim ehint i (focus: Subgoal.focus) =
+fun b_assert_conj_foc_tac global_assms forall_and_exists_thm_tuple vc_elim ehint i (focus: Subgoal.focus) =
 let 
   val (red :: vc :: _) = #prems(focus)
   val ctxt = #context(focus)
 in
- (b_assert_base_tac ctxt (@{thm assert_ml} OF [red]) (@{thm conjunct1} OF [vc]) global_assms forall_poly_thm ehint i) THEN
+ (b_assert_base_tac ctxt (@{thm assert_ml} OF [red]) (@{thm conjunct1} OF [vc]) global_assms forall_and_exists_thm_tuple ehint i) THEN
   (resolve_tac ctxt [(vc_elim OF [vc])] i)  
   handle THM _ => no_tac 
 end
 
-fun b_assert_conj_tac ctxt global_assms forall_poly_thm vc_elim ehint =
-  (Subgoal.FOCUS (b_assert_conj_foc_tac global_assms forall_poly_thm vc_elim ehint 1) ctxt 1)  THEN
+fun b_assert_conj_tac ctxt global_assms forall_and_exists_thm_tuple vc_elim ehint =
+  (Subgoal.FOCUS (b_assert_conj_foc_tac global_assms forall_and_exists_thm_tuple vc_elim ehint 1) ctxt 1)  THEN
   eresolve0_tac [thin_rl] 1 THEN
   eresolve0_tac [thin_rl] 1
 
-fun b_assert_no_conj_foc_tac global_assms forall_poly_thm ehint i (focus: Subgoal.focus) =
+fun b_assert_no_conj_foc_tac global_assms forall_and_exists_thm_tuple ehint i (focus: Subgoal.focus) =
 let 
   val (red :: vc :: _) = #prems(focus) 
   val ctxt = #context(focus)
 in
- (b_assert_base_tac ctxt (@{thm assert_ml} OF [red]) vc global_assms forall_poly_thm ehint i)
+ (b_assert_base_tac ctxt (@{thm assert_ml} OF [red]) vc global_assms forall_and_exists_thm_tuple ehint i)
   handle THM _ => no_tac 
 end
 
-fun b_assert_no_conj_tac ctxt global_assms forall_poly_thm ehint =
-  (Subgoal.FOCUS (b_assert_no_conj_foc_tac global_assms forall_poly_thm ehint 1) ctxt 1)
+fun b_assert_no_conj_tac ctxt global_assms forall_and_exists_thm_tuple ehint =
+  (Subgoal.FOCUS (b_assert_no_conj_foc_tac global_assms forall_and_exists_thm_tuple ehint 1) ctxt 1)
 \<close>
 
 ML \<open>
@@ -211,29 +241,29 @@ ML \<open>
 
 fun boogie_vc_tac ctxt _ _ ([]: (VcHint * (ExprHint option)) list) =
   TRY (eresolve_tac ctxt [@{thm nil_cmd_elim}] 1 THEN asm_full_simp_tac ctxt 1)
-| boogie_vc_tac ctxt global_assms forall_poly_thm (x::xs) = 
+| boogie_vc_tac ctxt global_assms forall_and_exists_thm_tuple (x::xs) = 
   (case x of
   (* assume statement normal *)
-    (AssumeConjR 0, ehint) => b_assume_simple_tac ctxt global_assms forall_poly_thm (fn (vc) => @{thm impE} OF [vc]) ehint 3
+    (AssumeConjR 0, ehint) => b_assume_simple_tac ctxt global_assms forall_and_exists_thm_tuple (fn (vc) => @{thm impE} OF [vc]) ehint 3
   | (AssumeConjR n, ehint) => 
      if n = 1 then
-        b_assume_simple_tac ctxt global_assms forall_poly_thm (fn (vc) => @{thm imp_conj_elim} OF [vc]) ehint 3
+        b_assume_simple_tac ctxt global_assms forall_and_exists_thm_tuple (fn (vc) => @{thm imp_conj_elim} OF [vc]) ehint 3
      else
-       b_assume_conjr_tac ctxt global_assms forall_poly_thm ehint n
+       b_assume_conjr_tac ctxt global_assms forall_and_exists_thm_tuple ehint n
   (* assert statement normal *)
-  | (AssertNoConj, ehint) => b_assert_no_conj_tac ctxt global_assms forall_poly_thm ehint
-  | (AssertConj, ehint) => b_assert_conj_tac ctxt global_assms forall_poly_thm (@{thm conj_elim_2}) ehint
-  | (AssertSub, ehint) => b_assert_conj_tac ctxt global_assms forall_poly_thm (@{thm conj_imp_elim}) ehint 
+  | (AssertNoConj, ehint) => b_assert_no_conj_tac ctxt global_assms forall_and_exists_thm_tuple ehint
+  | (AssertConj, ehint) => b_assert_conj_tac ctxt global_assms forall_and_exists_thm_tuple (@{thm conj_elim_2}) ehint
+  | (AssertSub, ehint) => b_assert_conj_tac ctxt global_assms forall_and_exists_thm_tuple (@{thm conj_imp_elim}) ehint 
   (* special cases *)
   | (AssumeFalse, _) => (eresolve_tac ctxt [@{thm assume_false_cmds}] 1) THEN (ALLGOALS (asm_full_simp_tac ctxt))
-  | (AssumeNot, ehint) => b_assume_simple_tac ctxt global_assms forall_poly_thm (fn (vc) => @{thm imp_not_elim} OF [vc]) ehint 0 THEN 
+  | (AssumeNot, ehint) => b_assume_simple_tac ctxt global_assms forall_and_exists_thm_tuple (fn (vc) => @{thm imp_not_elim} OF [vc]) ehint 0 THEN 
       TRY (ALLGOALS (asm_full_simp_tac ctxt))
   | (AssertFalse, _) => SOLVED' (asm_full_simp_tac ctxt) 1
   | (AssumeTrue, _) => (eresolve_tac ctxt [@{thm assume_true_cmds}] 1) THEN (asm_full_simp_tac ctxt 1) THEN
                   rotate_tac 1 1
   | (AssertTrue, _) => (eresolve_tac ctxt [@{thm assert_true_cmds}] 1) THEN (rotate_tac 1 1)
   ) THEN
-   boogie_vc_tac ctxt global_assms forall_poly_thm xs
+   boogie_vc_tac ctxt global_assms forall_and_exists_thm_tuple xs
 \<close>
 
 end
